

# *Multivariable Calculus- Semester III*

Durga Deshmukh

November 6, 2025

# Limits

## Definition

Limit for multi-variable functions is given as,

$\lim_{(x,y) \rightarrow (a,b)} f(x) = l$ , given any  $\epsilon > 0$ ,  $\exists \delta > 0$  such that  $\text{mod } f(x) - l < \epsilon$   
for  $0 < \sqrt{(x-a)^2 + (y-b)^2} < \delta$

If a limit exists then it is unique.

---

### Example:

Q. Find limit.

a)  $\lim_{(x,y) \rightarrow (2,3)} \frac{x^2 y}{x^2 + y^2}$

$\rightarrow$

$$\lim_{(x,y) \rightarrow (2,3)} \frac{x^2 y}{x^2 + y^2} = \frac{(2)^2(3)}{(2)^2 + (3)^2} = \frac{4(3)}{4+9} = \frac{12}{13}$$

$\lim_{(x,y) \rightarrow (2,3)} \frac{x^2 y}{x^2 + y^2} = \frac{12}{13}$
--

---

b)  $\lim_{(x,y) \rightarrow (0,0)} \frac{x-y}{x+y}$

$\rightarrow$

We know that, if a limit exists then it is unique along all paths.

Along,  $x = 0$

$$\frac{x-y}{x+y} = \frac{-y}{y} = -1$$

$$\lim_{(x,y) \rightarrow (0,0)} \frac{x-y}{x+y} = -1$$

Along,  $y = 0$

$$\frac{x-y}{x+y} = \frac{x}{x} = 1$$

$$\lim_{(x,y) \rightarrow (0,0)} \frac{x-y}{x+y} = 1$$

Along two different paths there are two different limits. But, we know if limit exists then it is unique.

$$\therefore \lim_{(x,y) \rightarrow (0,0)} \frac{x-y}{x+y} \text{ does not exist.}$$


---

## ***Important***

### ***Open disk or open ball***

Open disk or open ball is given as,

$$B((a, b), \delta) = \left\{ (x, y) \in \mathbb{R}^2 \mid \sqrt{(x-a)^2 + (y-b)^2} < \delta \right\}$$


---

### ***Theorem***

Let  $\lim_{(x,y) \rightarrow (a,b)} f(x, y) = 0$  and  $g(x,y)$  is bounded in some  $B((a, b), \delta)$  then,  
 $\lim_{(x,y) \rightarrow (a,b)} f(x, y) \cdot g(x, y) = 0$

---

### **Example:**

Q. Find limit if exists.

a)  $\lim_{(x,y) \rightarrow (0,0)} \frac{x^2 y^2}{x^2 + y^2}$   
 $\rightarrow$

Here,

$$\frac{x^2 y^2}{x^2 + y^2} = \left( \frac{x^2}{x^2 + y^2} \right) y^2$$

We know,

$$\lim_{(x,y) \rightarrow (0,0)} y^2 = 0$$

$$0 < y^2 \rightarrow x^2 \leq x^2 + y^2 \rightarrow 0 \leq \frac{x^2}{x^2 + y^2} \leq 1$$

By the theorem,

Let  $\lim_{(x,y) \rightarrow (a,b)} f(x, y) = 0$  and  $g(x,y)$  is bounded in some  $B((a, b), \delta)$  then,

$$\lim_{(x,y) \rightarrow (a,b)} f(x, y) \cdot g(x, y) = 0$$

$$\lim_{(x,y) \rightarrow (0,0)} \frac{x^2 y^2}{x^2 + y^2} = 0$$


---

b)  $\lim_{(x,y) \rightarrow (0,0)} \frac{x^3 + y^3}{x^2 + y^2}$   
 $\rightarrow$

Here,

$$\frac{x^3 + y^3}{x^2 + y^2} = \frac{x^3}{x^2 + y^2} + \frac{y^3}{x^2 + y^2} = x \left( \frac{x^2}{x^2 + y^2} \right) + y \left( \frac{y^2}{x^2 + y^2} \right)$$

We know,

$$\lim_{(x,y) \rightarrow (0,0)} x = 0 \text{ and } \lim_{(x,y) \rightarrow (0,0)} y = 0$$

$$0 \leq \frac{x^2}{x^2+y^2} \leq 1 \text{ and } 0 \leq \frac{y^2}{x^2+y^2} \leq 1$$

By the theorem,

Let  $\lim_{(x,y) \rightarrow (a,b)} f(x,y) = 0$  and  $g(x,y)$  is bounded in some  $B((a,b), \delta)$  then,

$$\lim_{(x,y) \rightarrow (a,b)} f(x,y) \cdot g(x,y) = 0$$

$$\lim_{(x,y) \rightarrow (0,0)} x \left( \frac{x^2}{x^2+y^2} \right) = 0 \text{ and } \lim_{(x,y) \rightarrow (0,0)} y \left( \frac{y^2}{x^2+y^2} \right) = 0$$

$$\therefore \lim_{(x,y) \rightarrow (0,0)} \frac{x^3 + y^3}{x^2 + y^2} = 0$$

$$\text{c) } \lim_{(x,y) \rightarrow (0,0)} \frac{xy}{\sqrt{x^2+y^2}}$$

$\rightarrow$

Use, polar co-ordinates,  $x = r \cos \theta$  and  $y = r \sin \theta$

$$\therefore r = \sqrt{x^2 + y^2}$$

$$\lim_{(x,y) \rightarrow (0,0)} \frac{xy}{\sqrt{x^2+y^2}} = \lim_{r \rightarrow 0} \frac{(r \cos \theta)(r \sin \theta)}{r} = \lim_{r \rightarrow 0} r \cos \theta \sin \theta = 0$$

$$\therefore \lim_{(x,y) \rightarrow (0,0)} \frac{xy}{\sqrt{x^2 + y^2}} = 0$$

# Continuity

## Definition

A function  $f(x,y)$  is said to be continuous at  $(a,b)$  if,  
 $\lim_{(x,y) \rightarrow (a,b)} f(x,y) = f(a,b)$

---

**Example:** Q. Discuss the continuity of the following:

a)  $f(x,y) = \frac{xy}{x^2+y^2}, (x,y) \neq (0,0), f(0,0) = 0$

$\rightarrow$

We check limit along various paths,

Along  $x = 0$ ,

$$f(x,y) = 0 \implies \lim_{(x,y) \rightarrow (0,0)} f(x,y) = 0$$

Along  $x = y$ ,

$$f(x,y) = \frac{x^2}{2x^2} = \frac{1}{2} \implies \lim_{(x,y) \rightarrow (0,0)} f(x,y) = \frac{1}{2}$$

Along two different paths there are two different limits. But, we know if limit exists then it is unique.

$\therefore \lim_{(x,y) \rightarrow (0,0)} f(x,y)$  doesn't exist.

$\therefore f(x,y)$  is discontinuous at  $(0,0)$

---

# *Partial Derivatives*

## *Definition*

First order partial derivatives are given as,

$$f_x = \frac{\partial f}{\partial x}(a, b) = \lim_{h \rightarrow 0} \frac{f(a+h, b) - f(a, b)}{h}$$

$$f_y = \frac{\partial f}{\partial y}(a, b) = \lim_{k \rightarrow 0} \frac{f(a, b+k) - f(a, b)}{k}$$

Second order partial derivatives are given as,

$$f_{xx} = \frac{\partial^2 f}{\partial x^2}(a, b) = \lim_{h \rightarrow 0} \frac{f_x(a+h, b) - f_x(a, b)}{h}$$

$$f_{xy} = \frac{\partial^2 f}{\partial y \partial x}(a, b) = \lim_{k \rightarrow 0} \frac{f_y(a, b+k) - f_y(a, b)}{k}$$

$$f_{yx} = \frac{\partial^2 f}{\partial x \partial y}(a, b) = \lim_{h \rightarrow 0} \frac{f_y(a, b+h) - f_y(a, b)}{h}$$

$$f_{yy} = \frac{\partial^2 f}{\partial y^2}(a, b) = \lim_{k \rightarrow 0} \frac{f_y(a, b+k) - f_y(a, b)}{k}$$

---

### **Example:**

Q. Find first order partial derivatives:

a)  $f(x, y) = \tan^{-1}\left(\frac{x}{y}\right)$

→

We know, derivative of;

$$\tan^{-1}(x) = \frac{1}{1+x^2}$$

So,

$$f_x = \frac{\partial f}{\partial x} = \frac{y}{x^2+y^2}$$

$$f_y = \frac{\partial f}{\partial y} = \frac{(-x)}{x^2+y^2}$$

---

b)  $f(x, y) = \frac{xy}{x^2+y^2}, (x, y) \neq (0, 0), f(0, 0) = 0$

→

First order derivatives are,

$$f_x = \frac{\partial f}{\partial x} = \lim_{h \rightarrow 0} \frac{f(h, 0) - f(0, 0)}{h} = 0$$

$$f_y = \frac{\partial f}{\partial y} = \lim_{k \rightarrow 0} \frac{f(0, k) - f(0, 0)}{k} = 0$$

$$\therefore f_x = 0, f_y = 0$$

---

Q. Find all first and second order partial derivatives of f at (1,2).

$$f = 3x^3 + 2xy^2 + y^3$$

→

$$f = 3x^3 + 2xy^2 + y^3$$

$$f_x = 9x^2 + 2y^2 \implies f_x(1, 2) = 9 + 8 = 17$$

$$f_{xx} = 18x \implies f_{xx}(1, 2) = 18$$

$$f_{xy} = 4y \implies f_{xy}(1, 2) = 8$$

$$f_y = 4xy + 3y^2 \implies f_y(1, 2) = 8 + 12 = 20$$

$$f_{yy} = 4x + 6y \implies f_{yy}(1, 2) = 4 + 12 = 16$$

$$f_{yx} = 4y \implies f_{yx}(1, 2) = 8$$


---

Q. Show that  $\frac{\partial u}{\partial x} + \frac{\partial u}{\partial y} = \frac{2}{x+y}$  where,  $u = \log(x^3 + y^3 - x^2y - xy^2)$

→

$$u = \log(x^3 + y^3 - x^2y - xy^2)$$

$$\frac{\partial u}{\partial x} = \frac{3x^2 - 2xy - y^2}{x^3 + y^3 - x^2y - xy^2}$$

$$\frac{\partial u}{\partial y} = \frac{3y^2 - x^2 - 2xy}{x^3 + y^3 - x^2y - xy^2}$$

Now,

$$\text{LHS} = \frac{\partial u}{\partial x} + \frac{\partial u}{\partial y}$$

$$= \frac{3x^2 - 2xy - y^2 + 3y^2 - x^2 - 2xy - x^2}{x^3 + y^3 - x^2y - xy^2}$$

$$= \frac{2(x-y)^2}{(x+y)(x-y)^2}$$

$$= \frac{2}{(x+y)}$$

$$= \text{RHS}$$

$$\therefore \frac{\partial u}{\partial x} + \frac{\partial u}{\partial y} = \frac{2}{x+y}$$


---

## ***Laplace equation***

Laplace equation is given as,

$$\frac{\partial^2 u}{\partial x^2} + \frac{\partial^2 u}{\partial y^2} = 0$$

–**Harmonic function:**

If  $u(x, y)$  satisfies the Laplace equation, then  $u$  is called as a harmonic function.

---

**Example:**

Q. Check whether the following are harmonic or not:

a)  $u(x, y) = x^2 + y^2$

→

$$f_x = \frac{\partial u}{\partial x} = 2x$$

$$f_{xx} = \frac{\partial^2 u}{\partial x^2} = 2$$

$$f_y = \frac{\partial u}{\partial y} = 2y$$

$$f_{yy} = \frac{\partial^2 u}{\partial y^2} = 2$$

Now,

$$\frac{\partial^2 u}{\partial x^2} + \frac{\partial^2 u}{\partial y^2} = 2 + 2 = 4 \neq 0$$

∴  $u(x, y) = x^2 + y^2$  is not a harmonic function.

---

b)  $u(x, y) = \log(x^2 + y^2)$

→

$$f_x = \frac{\partial u}{\partial x} = \frac{2x}{x^2 + y^2}$$

$$f_{xx} = \frac{\partial^2 u}{\partial x^2} = \frac{2(y^2 - x^2)}{(x^2 + y^2)^2}$$

$$f_y = \frac{\partial u}{\partial y} = \frac{2y}{x^2 + y^2}$$

$$f_{yy} = \frac{\partial^2 u}{\partial y^2} = \frac{2(x^2 - y^2)}{(x^2 + y^2)^2}$$

Now,

$$\frac{\partial^2 u}{\partial x^2} + \frac{\partial^2 u}{\partial y^2} = \frac{2(y^2 - x^2)}{(x^2 + y^2)^2} + \frac{2(x^2 - y^2)}{(x^2 + y^2)^2} = \frac{2(y^2 - x^2) + 2(x^2 - y^2)}{(x^2 + y^2)^2}$$

∴  $u(x, y) = \log(x^2 + y^2)$  is a harmonic function.

---

Q. Show that  $\frac{\partial^2 f}{\partial y \partial x} = \frac{\partial^2 f}{\partial x \partial y}$  where  $f = \tan^{-1}\left(\frac{y}{x}\right)$ .

→

$$\frac{\partial f}{\partial x} = \frac{(-y)}{x^2 + y^2} \implies \frac{\partial^2 f}{\partial y \partial x} = \frac{y^2 - x^2}{(x^2 + y^2)^2}$$

$$\frac{\partial f}{\partial x} = \frac{x}{x^2 + y^2} \implies \frac{\partial^2 f}{\partial x \partial y} = \frac{y^2 - x^2}{(x^2 + y^2)^2}$$

$$\therefore \frac{\partial^2 f}{\partial y \partial x} = \frac{\partial^2 f}{\partial x \partial y}$$

---

Q. Show that  $x \frac{\partial v}{\partial x} - y \frac{\partial v}{\partial y} = y^2 v^3$  where  $v = (1 - 2xy + y^2)^{-1/2}$

→

$$\frac{\partial v}{\partial x} = y(1 - 2xy + y^2)^{-3/2}$$

$$\frac{\partial v}{\partial y} = (x - y)(1 - 2xy + y^2)^{-3/2}$$

Now,

$$\text{LHS} = x \frac{\partial v}{\partial x} - y \frac{\partial v}{\partial y} = xy(1 - 2xy + y^2)^{-3/2} - y(x - y)(1 - 2xy + y^2)^{-3/2}$$



$$\begin{aligned}
&= xy(1 - 2xy + y^2)^{-3/2} - (xy - y^2)(1 - 2xy + y^2)^{-3/2} \\
&= xy(1 - 2xy + y^2)^{-3/2} - xy(1 - 2xy + y^2)^{-3/2} + y^2(1 - 2xy + y^2)^{-3/2} \\
&= y^2(1 - 2xy + y^2)^{-3/2} \\
&= y^2 v^3 \\
&= \text{RHS} \\
\therefore x \frac{\partial v}{\partial x} - y \frac{\partial v}{\partial y} &= y^2 v^3
\end{aligned}$$


---

Q. Suppose  $z = \sin(nx) \cdot \cos(y^2)$  satisfies,  
 $y^3 \cdot \frac{\partial^2 z}{\partial x^2} - y \frac{\partial^2 z}{\partial y^2} + \frac{\partial z}{\partial y} = 0$  for all (x,y). Find n.  
 $\rightarrow$

Here,

$$\begin{aligned}
\frac{\partial z}{\partial x} &= \cos(nx) \cdot n \cdot \cos(y^2) = n \cos(nx) \cdot \cos(y^2) \\
\therefore \frac{\partial^2 z}{\partial x^2} &= -n^2 \cdot \sin(nx) \cdot \cos(y^2) \\
\frac{\partial z}{\partial y} &= -\sin(nx) \cdot \sin(y^2) \cdot 2y = -2y \sin(nx) \cdot \sin(y^2) \\
\therefore \frac{\partial^2 z}{\partial y^2} &= -2 \sin(nx) \sin(y^2) - 4y^2 \sin(nx) \cos(y^2) \\
y^3 \cdot \frac{\partial^2 z}{\partial x^2} - y \frac{\partial^2 z}{\partial y^2} + \frac{\partial z}{\partial y} &= y^3(-n^2 \cdot \sin(nx) \cdot \cos(y^2)) - y(-2 \sin(nx) \sin(y^2) - 4y^2 \sin(nx) \cos(y^2)) + (-2y \sin(nx) \cdot \sin(y^2)) = 0
\end{aligned}$$

Hence, proved.

---

Q.  $f(x, y) = \frac{xy^3}{x^2 + y^2}$  if (x,y)  $\neq$  0,  $f(0,0) = 0$ .

Show that  $f_{xy}(0,0) \neq f_{yx}(0,0)$

$$\begin{aligned}
&\rightarrow \\
\frac{\partial^2 f}{\partial y \partial x}(0,0) &= \lim_{k \rightarrow 0} \frac{f_x(0,k) - f_x(0,0)}{k} \\
\Rightarrow f_x(0,k) &= \lim_{h \rightarrow 0} \frac{f(h,k) - f(0,k)}{h} = k \\
\Rightarrow f_x(0,k) &= k \\
\Rightarrow f_x(0,0) &= \lim_{h \rightarrow 0} \frac{f(h,0) - f(0,0)}{h} = 0 \\
\therefore \frac{\partial^2 f}{\partial y \partial x}(0,0) &= \lim_{k \rightarrow 0} \frac{f_x(0,k) - f_x(0,0)}{k} = \lim_{k \rightarrow 0} \frac{k-0}{k} = 1 \\
\therefore \frac{\partial^2 f}{\partial y \partial x}(0,0) &= 1
\end{aligned}$$

Now,

$$\begin{aligned}
\frac{\partial^2 f}{\partial x \partial y}(0,0) &= \lim_{h \rightarrow 0} \frac{f_y(h,0) - f_y(0,0)}{h} \\
\Rightarrow f_y(h,0) &= \lim_{k \rightarrow 0} \frac{f(h,k) - f(0,k)}{k} = 0 \\
\Rightarrow f_y(h,0) &= 0 \\
\Rightarrow f_y(0,0) &= \lim_{k \rightarrow 0} \frac{f(0,k) - f(0,0)}{k} = 0 \\
\therefore \frac{\partial^2 f}{\partial x \partial y}(0,0) &= \lim_{h \rightarrow 0} \frac{f_y(h,0) - f_y(0,0)}{h} = \lim_{h \rightarrow 0} \frac{0-0}{h} = 0 \\
\therefore \frac{\partial^2 f}{\partial x \partial y}(0,0) &= 0
\end{aligned}$$

$$\therefore f_{xy}(0,0) \neq f_{yx}(0,0)$$


---

## ***Differentiability***

### ***Definition***

We say that  $f(x, y)$  is differentiable at  $(a, b)$  if there exist  $c_1, c_2 \in \mathbb{R}$  such that

$$\lim_{(h,k) \rightarrow (0,0)} \frac{f(a+h, b+k) - f(a, b) - (hc_1 + kc_2)}{\sqrt{h^2 + k^2}} = 0$$

### ***Theorem***

If  $f(x, y)$  is differentiable at  $(a, b)$  then:

- $f$  is continuous at  $(a, b)$
- Both first-order partial derivatives exist at  $(a, b)$

#### **Proof:**

I. To prove continuity:

Given differentiability, we add and subtract  $(hc_1 + kc_2)$ :

$$\implies \lim_{(h,k) \rightarrow (0,0)} \left[ \frac{f(a+h, b+k) - f(a, b) - (hc_1 + kc_2)}{\sqrt{h^2 + k^2}} \cdot \sqrt{h^2 + k^2} + (hc_1 + kc_2) \right] = 0$$

$\therefore f$  is continuous at  $(a, b)$

II. To prove existence of partial derivatives:

Put  $k = 0$ :

$$\lim_{h \rightarrow 0} \frac{f(a+h, b) - f(a, b)}{h} = c_1 \implies \frac{\partial f}{\partial x}(a, b) = c_1$$

Put  $h = 0$ :

$$\lim_{k \rightarrow 0} \frac{f(a, b+k) - f(a, b)}{k} = c_2 \implies \frac{\partial f}{\partial y}(a, b) = c_2$$

$\therefore$  Both partial derivatives exist.

#### **Example:**

Is  $f(x, y) = \frac{x^4 + y^4}{x^2 + y^2}$  for  $(x, y) \neq (0, 0)$  and  $f(0, 0) = 0$  differentiable at  $(0, 0)$

I. Continuity:

$$\frac{x^4 + y^4}{x^2 + y^2} = x \cdot \frac{x^3}{x^2 + y^2} + y \cdot \frac{y^3}{x^2 + y^2}$$

Since  $x, y \rightarrow 0$  and both fractions are bounded, by the product limit theorem:

$$\lim_{(x,y) \rightarrow (0,0)} \frac{x^4 + y^4}{x^2 + y^2} = 0$$

II. Partial derivatives:

$$f_x(0, 0) = \lim_{h \rightarrow 0} \frac{f(h, 0) - f(0, 0)}{h} = \lim_{h \rightarrow 0} \frac{h^4}{h} = 0$$

$$f_y(0, 0) = \lim_{k \rightarrow 0} \frac{f(0, k) - f(0, 0)}{k} = \lim_{k \rightarrow 0} \frac{k^4}{k} = 0$$

III. Differentiability check:

Since  $c_1 = c_2 = 0$ , we check:

$$\lim_{(h,k) \rightarrow (0,0)} \frac{f(h, k) - f(0, 0)}{\sqrt{h^2 + k^2}} = \lim_{(h,k) \rightarrow (0,0)} \frac{\frac{h^4 + k^4}{h^2 + k^2}}{\sqrt{h^2 + k^2}} = \lim_{(h,k) \rightarrow (0,0)} \frac{h^4 + k^4}{(h^2 + k^2)\sqrt{h^2 + k^2}} = 0$$

$\therefore f(x, y)$  is differentiable at  $(0, 0)$

## ***Applications***

### **Find approximate values**

We know that if  $f$  is differentiable at  $(a, b)$ ,

$$\lim_{(h,k) \rightarrow (0,0)} \left[ \frac{f(a + h, b + k) - f(a, b) - (f_x(a, b)h + f_y(a, b)k)}{\sqrt{h^2 + k^2}} \right]$$

For very small values of  $h$  and  $k$  in comparison to  $a$  and  $b$ ,

$$f(a + h, b + k) \approx f(a, b) + f_x(a, b)h + f_y(a, b)k$$

**Example:**

Find approximate value of:

$$\sqrt{(5.98)^2 + (8.01)^2}$$

→

$$\text{Let, } f(x, y) = \sqrt{x^2 + y^2}$$

Here,  $a = 6$ ,  $b = 8$ ,  $h = -0.02$ ,  $k = 0.01$

Now,

$$f(a + h, b + k) \approx f(a, b) + f_x(a, b)h + f_y(a, b)k$$

So,

$$f(a, b) = \sqrt{6^2 + 8^2} = \sqrt{36 + 64} = \sqrt{100} = 10$$

$$f_x(a, b) = \frac{2x}{2\sqrt{x^2 + y^2}} = \frac{x}{\sqrt{x^2 + y^2}} = \frac{6}{10} \cdot \frac{3}{5}$$

$$f_y(a, b) = \frac{2y}{2\sqrt{x^2 + y^2}} = \frac{y}{\sqrt{x^2 + y^2}} = \frac{8}{10} \cdot \frac{4}{5}$$

$$\therefore f(a + h, b + k) \approx 10 + \frac{3}{5} \times (-0.02) + \frac{4}{5} \times (0.01)$$

$$\approx 10 - 0.012 + 0.008$$

$$\approx 9.996$$

$$\therefore \sqrt{(5.98)^2 + (8.01)^2} \approx 9.996$$

---

## Chain rule

### Rule I:

If  $f(x, y)$  is differentiable function of  $x$  and  $y$ ;  $x = \phi(t)$  and  $y = \psi(t)$  are differentiable functions of  $t$  then,

For  $u = f(\phi(t), \psi(t))$ ,

$$\frac{du}{dt} = \frac{\partial u}{\partial x} \cdot \frac{dx}{dt} + \frac{\partial u}{\partial y} \cdot \frac{dy}{dt}$$

### Example:

Find  $\frac{du}{dt}$  at  $t = \frac{\pi}{2}$ ,  $\pi$

$$u = e^{xy^2}, x = t \cos t, y = t \sin t$$

→

By chain rule I,

If  $f(x, y)$  is differentiable function of  $x$  and  $y$ ;  $x = \phi(t)$  and  $y = \psi(t)$  are differentiable functions of  $t$  then,

For  $u = f(\phi(t), \psi(t))$ ,

$$\frac{du}{dt} = \frac{\partial u}{\partial x} \cdot \frac{dx}{dt} + \frac{\partial u}{\partial y} \cdot \frac{dy}{dt}$$

$$\begin{aligned}\frac{du}{dt} &= (y^2 e^{xy^2}) \cdot (-t \sin t + \cos t) + (2xy e^{xy^2}) \cdot (t \cos t + \sin t) \\ \frac{du}{dt} &= \sin t (2xy e^{xy^2} - ty^2 e^{xy^2}) + \cos t (y^2 e^{xy^2} + 2txy e^{xy^2}) \\ \therefore \frac{du}{dt} &= e^{xy^2} (\sin t (2xy - ty^2) + \cos t (y^2 + 2txy))\end{aligned}$$

Now,

$$\text{At } t = \frac{\pi}{2},$$

$$\frac{du}{dt} = \frac{-\pi^3}{2}$$

$$\text{At } t = \pi,$$

$$\frac{du}{dt} = 0$$

### Rule II:

If  $w = f(u, v)$  is a differentiable function of  $u$  &  $v$  and  $u = \phi(x, y)$  &  $v = \psi(x, y)$  are differentiable functions of  $x$  and  $y$  then,

For  $w = f(\phi(x, y), \psi(x, y)) =$ ,

$$\frac{\partial w}{\partial x} = \frac{\partial w}{\partial u} \cdot \frac{\partial u}{\partial x} + \frac{\partial w}{\partial v} \cdot \frac{\partial v}{\partial x}$$

$$\frac{\partial w}{\partial y} = \frac{\partial w}{\partial u} \cdot \frac{\partial u}{\partial y} + \frac{\partial w}{\partial v} \cdot \frac{\partial v}{\partial y}$$

### Example:

If  $z = \tan^{-1} \frac{x}{y}$ ,  $x = u + v$ ,  $y = u - v$ . Show that,

$$\frac{\partial z}{\partial u} + \frac{\partial z}{\partial v} = \frac{u - v}{u^2 + v^2}$$

→

By chain rule II,

If  $w = f(u, v)$  is a differentiable function of  $u$  &  $v$  and  $u = \phi(x, y)$  &  $v = \psi(x, y)$  are differentiable functions of  $x$  and  $y$  then,

For  $w = f(\phi(x, y), \psi(x, y)) =$ ,

$$\frac{\partial w}{\partial x} = \frac{\partial w}{\partial u} \cdot \frac{\partial u}{\partial x} + \frac{\partial w}{\partial v} \cdot \frac{\partial v}{\partial x}$$

$$\frac{\partial w}{\partial y} = \frac{\partial w}{\partial u} \cdot \frac{\partial u}{\partial y} + \frac{\partial w}{\partial v} \cdot \frac{\partial v}{\partial y}$$

$$\frac{\partial z}{\partial u} = \frac{y}{x^2+y^2} + \frac{-x}{x^2+y^2}$$

$$\frac{\partial z}{\partial v} = \frac{y}{x^2+y^2} + \frac{x}{x^2+y^2}$$

Now,

$$LHS = \frac{\partial z}{\partial u} + \frac{\partial w}{\partial v} = \frac{2y}{x^2+y^2} = \frac{u-v}{u^2+v^2} = RHS$$

Hence, proved.

---

## ***Homogeneous functions***

$f(x,y)$  is called "homogeneous function" of degree  $n$  if it can be expressed as,

$$f(tx, ty) = t^n \cdot f(x, y)$$

**Example:**

$$f(x,y) = x^2 - xy + y^2$$

→

Here,

$$f(tx,ty) = (tx)^2 - (tx)(ty) + (ty)^2$$

$$= t^2(x^2 - xy + y^2)$$

$$= t^2 \cdot f(x, y)$$

$$f(tx,ty) = t^2 \cdot f(x, y)$$

∴  $f(x,y)$  is a homogeneous function.

---

## ***Euler's theorem***

**Statement:**

If  $f(x,y)$  is a homogeneous function of  $x$  and  $y$  of degree  $n$  in an open region having continuous partial derivatives then,

$$x \cdot \frac{\partial f}{\partial x} + y \cdot \frac{\partial f}{\partial y} = nf$$

**Proof:**

Since,  $f(x,y)$  is a homogeneous function of  $x$  and  $y$  of degree  $n$ ,

$$f(x, y) = x^n \cdot f\left(\frac{y}{x}\right)$$

Differentiate the above equation wrt x,

$$\frac{\partial f}{\partial x} = nx^{n-1}.f\left(\frac{y}{x}\right) + x^n.f'\left(\frac{y}{x}\right)$$

$$\frac{\partial f}{\partial x} = nx^{n-1}.f\left(\frac{y}{x}\right) - x^{n-2}y.f'\left(\frac{y}{x}\right)$$

Multiply both sides by x,

$$x.\frac{\partial f}{\partial x} = nx^n.f\left(\frac{y}{x}\right) - y.x^{n-1}.f'\left(\frac{y}{x}\right)$$

Differentiate partially wrt y,

$$\frac{\partial f}{\partial y} = x^n.f'\left(\frac{y}{x}\right).\frac{1}{x}$$

$$\therefore \frac{\partial f}{\partial y} = x^{n-1}.f'\left(\frac{y}{x}\right)$$

Multiply both sides by y,

$$y.\frac{\partial f}{\partial y} = y.x^{n-1}.f'\left(\frac{y}{x}\right)$$

Add both,

$$x.\frac{\partial f}{\partial x} + y.\frac{\partial f}{\partial y} = nx^n.f\left(\frac{y}{x}\right)$$

$$x.\frac{\partial f}{\partial x} + y.\frac{\partial f}{\partial y} = nf$$

Hence, proved.

**Example:**

Find  $x.f_x + y.f_y$

$$f(x,y) = \frac{x^2+y^2}{x-y}$$

→

First,

$$f(tx,ty) = \frac{(tx)^2+(ty)^2}{(tx)-(ty)} = \frac{t^2(x^2+y^2)}{t(x-y)}$$

$$\therefore f(tx, ty) = t \cdot f(x, y)$$

So, f is a homogeneous function of degree 1.

$$\therefore x \cdot f_x + y \cdot f_y = f$$


---

### ***Critical point***

The point (a,b) is called as a critical point of f if,

$$f_x(a, b) = 0 \text{ and } f_y(a, b) = 0$$


---

### ***Important***

Let f be a real valued function defined on D containing point (a,b),

- If  $f(a,b) \geq f(x,y), \forall (x,y) \in D \implies f(a,b)$  is an absolute maximum.
  - If  $f(a,b) \leq f(x,y), \forall (x,y) \in D \implies f(a,b)$  is an absolute minimum.
  - If  $f(a,b) \geq f(x,y), \forall (x,y) \in N_\delta(a,b) \implies f(a,b)$  is a local maximum.
  - If  $f(a,b) \leq f(x,y), \forall (x,y) \in N_\delta(a,b) \implies f(a,b)$  is a local minimum.
- 

### ***Second derivative test***

Suppose a function f(x,y) and it's first & second order partial derivatives are continuous on  $N_\delta(a,b)$  and  $f_x(a,b) = 0$  &  $f_y(a,b) = 0$  then,

$$\text{Let, } A = f_{xx}(a,b), B = f_{xy}(a,b), C = f_{yy}(a,b)$$

$$\Delta = AC - B^2$$

If,

$$\Delta > 0 \text{ and } A < 0 \rightarrow f \text{ has local maximum at } (a,b)$$

$$\Delta > 0 \text{ and } A > 0 \rightarrow f \text{ has local minimum at } (a,b)$$

$$\Delta < 0 \rightarrow f \text{ has saddle point at } (a,b)$$

$$\Delta = 0 \rightarrow \text{Test fails}$$


---



## ***Lagrange's Method***

It is used to find extreme values of a function  $f(x,y,z)$  subject to another function  $g(x,y,z) = 0$   
Consider the equation,

$$\nabla f = \lambda \nabla g$$

$$\frac{\partial f}{\partial x} \vec{i} + \frac{\partial f}{\partial y} \vec{j} + \frac{\partial f}{\partial z} \vec{k} = \lambda \left( \frac{\partial g}{\partial x} \vec{i} + \frac{\partial g}{\partial y} \vec{j} + \frac{\partial g}{\partial z} \vec{k} \right)$$

---

## ***Directional Derivatives***

$$(\partial f)_{\vec{u}}(a, b) = \lim_{t \rightarrow 0} \frac{f(a + tu_1, b + tu_2) - f(a, b)}{t}$$

Formula:

$$(\partial f)_{\vec{u}}(\vec{a}) = \nabla f(\vec{a}) \cdot \vec{u}$$

**Partial derivatives are specific directional derivatives:** When  $\vec{u} = (1, 0)$ , we get:

$$(\partial f)_{\vec{u}}(a, b) = \frac{\partial f}{\partial x}(a, b)$$

When  $\vec{u} = (0, 1)$ , we get:

$$(\partial f)_{\vec{u}}(a, b) = \frac{\partial f}{\partial y}(a, b)$$

---

# *Integration*

To find area,

$$A = \iint_R 1 \, dA$$

To find volume,

$$V = \iiint_R 1 \, dV$$

**Example:**

Q. Find area of the region bounded by,

$y = x$  and  $y = x^2$

→

These curves intersect at: (0,0) and (1,1)

$$Area = \iint_R 1 \, dA = \int_0^1 \int_{x^2}^x 1 \, dy dx = \int_0^1 [x - x^2] dx = \frac{1}{6}$$

$$\therefore A = \frac{1}{6}$$

Q. Find volume of a tetrahedron bounded by  $x = 0, y = 0, z = 0, x + y + z = 1$

$$Volume = \iiint_R 1 \, dV = \int_0^1 \int_0^{1-x} \int_0^{1-y-x} 1 \, dz dy dx = \frac{1}{6}$$

$$\therefore V = \frac{1}{6}$$

---

Sometimes the process can be lengthy due to difficult or complex limits so substitute the following,

**Polar coordinates:**

When the given region is a disc or part of a disc; use polar co-ordinates;

$$x = r \cos \theta, y = r \sin \theta$$

Jacobian is:

$$J = \frac{\partial(x, y)}{\partial(r, \theta)} = r$$
$$\therefore \partial(x, y) = r \partial(r, \theta)$$

**Spherical polar coordinates:**

When the given region is a sphere or a part of sphere use,

$$x = r \sin \phi \cos \theta, y = r \sin \phi \sin \theta, z = r \cos \phi$$

Here,  $0 \leq \phi \leq \pi, 0 \leq \theta \leq 2\pi, 0 \leq r \leq a$

Jacobian is:

$$J = \frac{\partial(x, y, z)}{\partial(r, \phi, \theta)} = r^2 \sin \phi$$
$$\partial(x, y, z) = r^2 \sin \phi \partial(r, \phi, \theta)$$

**Cylindrical polar coordinates:**

When the given region is a cylinder use,

$$x = r \cos \theta, y = r \sin \theta, z = z$$

Here,  $0 \leq \theta \leq 2\pi, 0 \leq r \leq a$

Jacobian is:

$$J = \frac{\partial(x, y, z)}{\partial(r, \theta, z)} = r$$
$$\partial(x, y, z) = r \partial(r, \theta, z)$$

**Example:**

Q. Find volume of the sphere  $x^2 + y^2 + z^2 = a^2$

→

Using spherical polar coordinates,

$$Volume = \iiint_R 1 \, dV = \int_0^{2\pi} \int_0^\pi \int_0^a r^2 \sin \phi \, dr d\phi d\theta = \frac{4\pi a^3}{3}$$

$$\therefore V = \frac{4\pi a^3}{3}$$

---

# Algorithms

## Limits

### ***Find limit:***

- If not a indeterminate form, then substitute directly.
  - Check along various paths → If same value obtained then the limit exists and that value is the answer.
  - Use the product theorem
  - Use polar coordinates (mainly when  $\sqrt{x^2 + y^2}$  is present)
- 

## Continuity

### **Check if given function is continuous or not:**

- Write the definition
  - Find  $\lim_{(x,y) \rightarrow (a,b)} f(x, y)$
  - Compare with  $f(a,b)$   $\implies$  If equal then continuous
- 

## Partial Derivatives

### ***Find 1st order partial derivatives:***

- Directly differentiate if possible
  - Use definition
  - If asked put specific points and find values
- 

### ***Find 2nd order partial derivatives:***

- Find first order partial derivatives
  - Use them to find 2nd order by above methods.
-

**Check if a function is harmonic or not:**

- Write the Laplace equation
  - Check if the given function satisfies it.
  - If satisfies then it is harmonic
- 

**"Show that" questions:**

- Write the given function
  - Find all the required elements of LHS and RHS
  - Calculate LHS and RHS
  - Show that LHS = RHS
- 

**Find "n":**

- Use steps from above
  - Will get some equation → Solve it and get n
- 

**Show that  $f_{xy} \neq f_{yx}$ :**

- Find both separately using the methods mentioned above → Compare
- 

## Differentiability

**Check if differentiable at some point (a,b):**

- Check continuity at (a,b) → If continuous move further
- Check if both first order partial derivatives exist or not → If exists then move further
- Check if the definition is satisfied:

$$\lim_{(x,y) \rightarrow (a,b)} \frac{f(a+h, b+k) - f(a,b) - (hc_1 + kc_2)}{\sqrt{h^2 + k^2}} = 0$$

- If all of these satisfied then it is differentiable at (a,b)
- 

**Find approximate value:**

- Represent the given question in general terms
  - Use  $f(a+h, b+k) \approx f(a,b) + f_x(a,b)h + f_y(a,b)k$
  - Find the values required
  - Get the required value
-

**Questions on chain rule I:**

→ Here the question contains 1 function of 2 variables and 2 functions of 1 variable

→ Use the definition:

$$\frac{du}{dt} = \frac{\partial u}{\partial x} \frac{dx}{dt} + \frac{\partial u}{\partial y} \frac{dy}{dt}$$

→ Find using the definition

→ If asked at a specific point t then substitute and obtain the required value.

---

**Questions based on chain rule 2:**

→ Here the question contains 1 function of 2 variables and 2 functions of 2 variable

→ Use the definition:

$$\frac{\partial w}{\partial x} = \frac{\partial w}{\partial u} \cdot \frac{\partial u}{\partial x} + \frac{\partial w}{\partial v} \cdot \frac{\partial v}{\partial x}$$

$$\frac{\partial w}{\partial y} = \frac{\partial w}{\partial u} \cdot \frac{\partial u}{\partial y} + \frac{\partial w}{\partial v} \cdot \frac{\partial v}{\partial y}$$

→ Find both

---

**Check if homogeneous or not:**

→ Consider the definition:

$$f(tx, ty) = t^n f(x, y)$$

→ Check if the given function satisfies this → If yes, then it is homogeneous

---

**Questions based on Euler's theorem:**

**Proof:**

→ Write the statement → Differentiate partially wrt x and y → Add both

→ Make some changes and prove it.

**Find**  $x.f_x + y.f_y$ :

→ Check if homogeneous → Find n → Use  $x.f_x + y.f_y = n.f$

---

**Find critical points:**

Write definition → Find first order partial derivatives → Equate to 0 → Get equations → Solve them → Get solution → Put in  $f_y$  → Get critical points.

---

**Find local minima or maxima using 2nd derivative test:**

Find all first and second order partial derivatives → Find critical points → Consider points one by one and find  $\Delta$  → Check the second derivative conditions

---

**Word problems based on Lagrange's theorem:**

Assume variables and form equations according to the conditions → Classify  $g(x,y,z) = 0$  and  $f(x,y,z)$  from these → Find  $\nabla f$  and  $\nabla g$  → Use  $\nabla f = \lambda \nabla g$  → Find  $x,y,z$  in terms of  $\lambda$  → Find  $\lambda$  by re-substitution → Finally, get  $x,y$  and  $z$ .

---

**Rectangular box problem:**

Volume =  $xyz$  and Surface area =  $xy + 2xz + 2yz$  → Find 1st order partial derivatives → Find critical points → Use 2nd derivative test → Find minimum value → Dimensions are obtained.

---

**Find directional derivative:**

Use

$$(\partial f)_{\vec{u}}(a) = \nabla f(a) \cdot \vec{u}$$

→ Make sure that  $\vec{u}$  is unit vector

---

**Find tangent plane:**

A function and a point is given → Check if the point is on that plane → Find  $\nabla f(a)$  → It is normal to the tangent plane → Use  $\nabla f(a) \cdot ((x - x_1)\vec{i} + (y - y_1)\vec{j} + (z - z_1)\vec{k}) = 0$  → Gives the tangent plane equation

---

## Integration

**Evaluate limits:**

Similar to single integrals → First solve inner limit then the outer one → If order is changed then choose the appropriate limits

---

**Find area:**



Use:  $A = \iint_R 1 \, dA \rightarrow$  Find limits of R from a rough diagram  $\rightarrow$  Put them and solve A

---

***Find volume:***

Use:  $V = \iiint_R 1 \, dA \rightarrow$  Find limits of R from a rough diagram  $\rightarrow$  Put them and solve V

---

***If polar coordinates used:***

Proper substitution of function  $\rightarrow$  Remember the Jacobians correctly  $\rightarrow$  Remaining process similar to above

---